Util/VS2010/Dafny/DafnyLanguageService/Grammar.cs
@@ -16,7 +16,7 @@ namespace Demo
         StringLiteral stringLiteral = TerminalFactory.CreateCSharpString("String");
 
         this.MarkReservedWords(  // NOTE: these keywords must also appear once more below
-          "class", "ghost", "static", "var", "method", "datatype",
+          "class", "ghost", "static", "var", "method", "constructor", "datatype",
           "assert", "assume", "new", "this", "object", "refines", "replaces", "by",
           "unlimited", "module", "imports",
           "call", "if", "then", "else", "while", "invariant",
@@ -287,6 +287,7 @@ namespace Demo
           | "static"
           | "var"
           | "method"
+          | "constructor"
           | "datatype"
           | "assert"
           | "assume"
