Util/vim/syntax/dafny.vim
@@ -5,7 +5,7 @@
 
 syntax clear
 syntax case match
-syntax keyword dafnyFunction function method
+syntax keyword dafnyFunction function method constructor
 syntax keyword dafnyTypeDef class datatype 
 syntax keyword dafnyConditional if then else match case 
 syntax keyword dafnyRepeat foreach while
